\textbf{Definition:}
Aus der Funktion \ref{eq:uebertragung} stellt man die Matrizen auf:
    \begin{align*}
        \dot{\bs{x}} &= 
        \begin{bmatrix}
            0 &  \cdots & 0 &-a_n\\
            1 &\cdots & 0 & -a_{n-1} \\
            \vdots&\ddots&\vdots&\vdots\\
            0&\cdots&1&-a_1
        \end{bmatrix}\bs{x}+ 
        \begin{bmatrix}
            b_n \\ b_{n-1} \\ \vdots \\b_1
        \end{bmatrix} u \\
        y&= \begin{bmatrix}
            0 & \cdots & 0& 1
        \end{bmatrix} \bs{x}
    \end{align*}
    \begin{tcolorbox}[colback=white!10!white,colframe=gray!70!black,title=Umrechnungsregeln]
        \begin{align*}
            \bs{A}_O = \bs{A}_C^T &\hspace{0.3cm} \bs{B}_O = \bs{C}_C^T \\
            \bs{C}_O = \bs{B}_C^T   &\hspace{0.3cm} D_O = D_C
        \end{align*}
    
    \end{tcolorbox}
